\documentclass{article}
\usepackage{amsmath} % For align*
\usepackage{enumitem} % For customisable list labels
\usepackage{siunitx} % For units

\title{Advanced Engineering Mathematics Ordinary Differential Equations Formula Sheet}
\author{Chris Doble}
\date{February 2022}

\begin{document}

\tableofcontents

\section{First-order ODEs}

\textbf{Form:} IVP \[\frac{d y}{d x} = f(x, y)\] \[y(x_0) = y_0\] \\ \textbf{Test:} $f(x, y)$ and $\partial f / \partial y$ are continuous over $I$ \\ \textbf{Property:} A unique solution is guaranteed over $I$

\subsection{Separable Equations}

\textbf{Form:} \[\frac{d y}{d x} = g(x) h(y)\] \\ \textbf{Solution:} Divide by $h(y)$ then integrate with respect to $x$.

\begin{align*}
  \frac{d y}{d x}                          & = g(x) h(y)      \\
  \frac{1}{h(y)} \frac{d y}{d x}           & = g(x)           \\
  \int \frac{1}{h(y)} \frac{d y}{d x} \,dx & = \int g(x) \,dx \\
  \int \frac{1}{h(y)} \,dy                 & = \int g(x) \,dx \\
  H(y)                                     & = G(x) + c
\end{align*}

\subsection{Linear Equations}

\textbf{Form:} \[\frac{d y}{d x} + P(x) y = f(x)\] \\ \textbf{Solution:}

\begin{enumerate}
  \item Determine the integrating factor $e^{\int P(x) \,d x}$

  \item Multiply by the integrating factor

  \item Recognise that the left hand side of the equation is the derivative of the product of the integrating factor and $y$

  \item Integrate both sides of the equation

  \item Solve for $y$
\end{enumerate}

\subsection{Exact Equations}

\textbf{Form:} \[z = f(x, y) = c\] \[dz = \frac{\partial f}{\partial x} \,d x + \frac{\partial f}{\partial y} \,d y = M(x, y) \,d x + N(x, y) \,d y = 0\] \\ \textbf{Test:} \[\frac{\partial M}{\partial y} = \frac{\partial N}{\partial x}\] \\ \textbf{Solution:} \begin{enumerate}
  \item Integrate $M(x, y)$ with respect to $x$ to find an expression for $z = f(x, y)$

        \begin{align*}
          \frac{\partial f}{\partial x} & = M(x, y)                   \\
          f(x, y)                       & = \int M(x, y) \,d x + g(y)
        \end{align*}

  \item Differentiate $f(x, y)$ with respect to $y$ and equate it to $N(x, y)$ to find $g'(y)$

        \begin{align*}
          \frac{\partial f}{\partial y} = N(x, y) & = \frac{\partial}{\partial y} \int M(x, y) \,d x + g'(y)   \\
          g'(y)                                   & = N(x, y) - \frac{\partial}{\partial y} \int M(x, y) \,d x
        \end{align*}

  \item Integrate $g'(y)$ with respect to $y$ to find $g(y)$ and substitute it into $f(x, y)$

  \item Equate $f(x, y)$ with an unknown constant $c$
\end{enumerate} \textbf{Note:} The steps can be performed with $x$ and $y$ reversed, i.e. start by integrating $N(x, y)$ with respect to $y$, etc.

\subsection{Exact Equations with Integration Constant}

\textbf{Form:} \[M(x, y) \,d x + N(x, y) \,d y = 0\] \\ \textbf{Test:} $(M_y - N_x) / N$ is a function of $x$ alone or $(N_x - M_y) / M$ is a function of $y$ alone \\ \textbf{Solution:}

\begin{enumerate}
  \item Compute the integrating factor \[\mu(x) = e^{\int \frac{M_y - N_x}{N} \,d x}\] or \[\mu(y) = e^{\int \frac{N_x - M_y}{M} \,d y}\] as appropriate

  \item Multiple the equation by this factor

  \item The equation is now exact and can be solved as above
\end{enumerate}

\subsection{Homogeneous Equations}

\textbf{Form:} \[M(x, y) \,d x + N(x, y) \,d y = 0\] \\ \textbf{Test:} $M$ and $N$ are homogeneous functions of the same degree \\ \textbf{Solution:}

\begin{enumerate}
  \item Rewrite as \[M(x, y) = x^\alpha M(1, u) \text{ and } N(x, y) = x^\alpha N(1, u) \text{ where } u = y / x\] or \[M(x, y) = y^\alpha M(v, 1) \text{ and } N(x, y) = y^\alpha N(v, 1) \text{ where } v = x / y\]

  \item Substitute $y = u x$ and $d y = u \,d x + x \,d u$ or $x = v y$ and $d x = v \,d y + y \,d v$ as appropriate

  \item Solve the resulting first-order separable DE

  \item Substitude $u = y / x$ or $v = x / y$ as appropriate
\end{enumerate}

\subsection{Bernoulli's Equation}

\textbf{Form:} \[\frac{d y}{d x} + P(x) y = f(x) y^n\] \\ \textbf{Test:} $n \ne 0$ and $n \ne 1$ \\ \textbf{Solution:}

\begin{enumerate}
  \item Substitude $y = u^{1 / (1 - n)}$ and $\frac{d y}{d x} = \frac{d}{dx} (u^{1 / (1 - n)})$

  \item Solve the resulting linear equation

  \item Substitude $u = y^{1 - n}$
\end{enumerate}

\subsection{Reduction to Separation of Variables}

\textbf{Form:} \[\frac{d y}{d x} = f(A x + B y + C), B \ne 0\] \\ \textbf{Solution:} \begin{enumerate}
  \item Substitute \[A x + B y + C = u\]

  \item Solve the resulting separable equation

  \item Substitute \[u = A x + B y + C\]
\end{enumerate}

\subsection{Riccati's Equation}

\textbf{Form:} \[\frac{dy}{dx} = P(x) + Q(x) y + R(x) y^2\] \\ \textbf{Test:} You know a particular solution $y_1$ of the equation \\ \textbf{Solution:} \begin{enumerate}
  \item Substitute $y = y_1 + u$ and $y' = y_1' + u'$

  \item Solve the resulting Bernoulli equation

  \item Substitude $u = y - y_1$
\end{enumerate}

\end{document}