\documentclass{article}
\usepackage{amsmath} % For align*
\usepackage{amsfonts} % For open face letters
\usepackage{enumitem} % For customisable list labels
\usepackage{graphicx} % For images
\usepackage{siunitx} % For units
\graphicspath{{./images/}}

\setlist[enumerate, 1]{label={(\alph*)}}
\setlist[enumerate, 2]{label={(\roman*)}}

\title{University Physics with Modern Physics - Modern Physics by Young and Freedman Problems}
\author{Chris Doble}
\date{June 2023}

\begin{document}

\maketitle

\tableofcontents

\setcounter{section}{16}
\section{Temperature and Heat}

\subsection{Guided Practice}

\subsubsection{}

\begin{enumerate}
  \item

        \begin{align*}
          \Delta L & = \alpha L_0 \Delta T           \\
          \alpha   & = \frac{\Delta L}{L_0 \Delta T} \\
                   & = \qty{2.0e-5}{K^{-1}}
        \end{align*}

  \item

        \begin{align*}
          \Delta L & = \alpha L_0 \Delta T \\
                   & = \qty{-0.27}{mm}
        \end{align*}
\end{enumerate}

\subsubsection{}

\begin{align*}
  \Delta V_C              & = \beta V_{C0} \Delta T      \\
                          & = (\num{5.1e-5}) (250) (-70) \\
                          & = -\qty{0.893}{cm^3}         \\
  \Delta V_E              & = \beta V_{E0} \Delta T      \\
                          & = (\qty{75e-5}) (250) (-70)  \\
                          & = -\qty{13.1}{cm^3}          \\
  \Delta V_C - \Delta V_E & = \qty{12.2}{cm^3}           \\
                          & = \qty{12.2}{mL}
\end{align*}

\subsubsection{}

\begin{align*}
  \frac{\Delta L}{L_0}            & = \alpha \Delta T                                    \\
  Y                               & = \frac{F / A}{\Delta L / L_0}                       \\
  \frac{\Delta L}{L_0}            & = \frac{F}{A Y}                                      \\
  \alpha \Delta T + \frac{F}{A Y} & = 0                                                  \\
  \frac{F}{A Y}                   & = -\alpha \Delta T                                   \\
  F                               & = -\alpha A Y \Delta T                               \\
                                  & = -(\num{2.0e-5}) (\pi 0.005^2) (\num{9.0e10}) (-12) \\
                                  & = \qty{1.70e3}{N}
\end{align*}

Tensile

\subsubsection{}

\begin{align*}
  \Delta L                  & = \alpha_A L_A \Delta T + \alpha_B L_B \Delta T                                       \\
  \frac{\Delta L}{\Delta T} & = \alpha_A L_A + \alpha_B (L - L_A)                                                   \\
                            & = (\alpha_A - \alpha_B) L_A + \alpha_B L                                              \\
  L_A                       & = \frac{1}{\alpha_A - \alpha_B} \left( \frac{\Delta L}{\Delta T} - \alpha_B L \right)
\end{align*}

\subsubsection{}

\begin{align*}
  0      & = m_{Al} c_{Al} \Delta T_{Al} + m_W c_W \Delta T_W \\
         & = m_{Al} c_{Al} (T - T_{Al}) + m_W c_W (T - T_W)   \\
  m_{Al} & = -\frac{m_W c_W (T - T_W)}{c_{Al} (T - T_{Al})}   \\
         & = \qty{0.20}{kg}
\end{align*}

\subsubsection{}

\begin{align*}
  0 & = m_I L_f + m_C c_C \Delta T \\
    & = m_I L_f - m_C c_C T        \\
  T & = \frac{m_I L_f}{m_C c_C}    \\
    & = \qty{14.0}{\degree C}
\end{align*}

\subsubsection{}

\begin{align*}
  0   & = m_I L_F + m_I c_I \Delta T_I + m_E c_E \Delta T_E \\
      & = m_I (L_F + c_I \Delta T_I) + m_E c_E \Delta T_E   \\
  m_I & = -\frac{m_E c_E \Delta T_E}{L_F + c_I \Delta T_I}  \\
      & = \qty{0.176}{kg}
\end{align*}

\subsubsection{}

Cooling the silver to $\qty{0}{\degree C}$ would take \[Q = m c \Delta T = \qty{92137.5}{J}\] whereas melting all of the ice would take \[Q = m L_f = \qty{83500}{J}\] so all of the ice will melt.

\begin{align*}
  0 & = m_{Ag} c_{Ag} \Delta T_{Ag} + m_I L_f + m_I c_I \Delta T_I + m_I c_W \Delta T_W \\
    & = m_{Ag} c_{Ag} (T - T_{Ag}) + m_I L_F - m_I c_I T_I + m_I c_W T                  \\
    & = (m_{Ag} c_{Ag} + m_I c_W) T - m_{Ag} c_{Ag} T_{Ag} + m_I L_F - m_I c_I T_I      \\
  T & = \frac{m_{Ag} c_{Ag} T_{Ag} + m_I c_I T_I - m_I L_F}{m_{Ag} c_{Ag} + m_I c_W}    \\
    & = \qty{3.31}{\degree C}
\end{align*}

\subsubsection{}

\begin{enumerate}
  \item

        \begin{align*}
          H & = k A \frac{T_H - T_C}{L}   \\
          k & = \frac{H L}{A (T_H - T_C)} \\
            & = \qty{0.754}{W/(m.K)}
        \end{align*}

  \item \[H = k A \frac{T_H - T_C}{L} = \qty{733}{W}\]
\end{enumerate}

\subsubsection{}

\begin{enumerate}
  \item

        \begin{align*}
          L      & = \qty{0.250}{m}          \\
          A      & = \qty{2.00e-4}{m^2}      \\
          k_B    & = \qty{109.0}{W/(m.K)}    \\
          k_{Pb} & = \qty{34.7}{W/(m.K)}     \\
          T      & = \qty{185}{\degree C}    \\
          H      & = \qty{6.00}{W}           \\ \\
          H      & = k_B A \frac{T_H - T}{L} \\
          T_H    & = \frac{H L}{k_B A} + T   \\
                 & = \qty{254}{\degree C}
        \end{align*}

  \item

        \begin{align*}
          H   & = k_{Pb} A \frac{T - T_C}{L} \\
          T_C & = T - \frac{H L}{k_{Pb} A}   \\
              & = \qty{-31.1}{\degree C}
        \end{align*}
\end{enumerate}

\subsubsection{}

\begin{align*}
  H         & = 4 \pi (k r_E)^2 e \sigma T^4                      \\
  (k r_E)^2 & = \frac{H}{4 \pi e \sigma T^4}                      \\
  k         & = \frac{1}{r_E} \sqrt{\frac{H}{4 \pi e \sigma T^4}} \\
            & = 1.70
\end{align*}

\subsubsection{}

\begin{enumerate}
  \item

        \begin{align*}
          H                  & = A e \sigma T^4                \\
                             & = \pi r^2 \sigma T^4            \\
          H                  & = k A \frac{T_H - T_C}{L}       \\
                             & = k \pi r^2 \frac{T_H - T_C}{L} \\
          \pi r^2 \sigma T^4 & = k \pi r^2 \frac{T_H - T_C}{L} \\
          T_H                & = \frac{L \sigma T^4}{k} + T_C  \\
                             & = \qty{14.26}{K}
        \end{align*}

  \item

        \begin{align*}
          H                  & = m L_f                          \\
          \pi r^2 \sigma T^4 & = m L_f                          \\
          m                  & = \frac{\pi r^2 \sigma T^4}{L_f} \\
                             & = \qty{1.19e-4}{kg/s}            \\
                             & = \qty{0.427}{kg/h}
        \end{align*}
\end{enumerate}

\subsection{Exercises and Problems}

\setcounter{subsubsection}{14}
\subsubsection{}

\begin{align*}
  \Delta V             & = \beta V_0 \Delta T               \\
  \frac{\Delta V}{V_0} & = \beta (T - T_0)                  \\
  T                    & = T_0 + \frac{\Delta V}{\beta V_0} \\
                       & = \qty{49}{\degree C}
\end{align*}

\setcounter{subsubsection}{24}
\subsubsection{}

\begin{align*}
  Q & = (m_{Al} c_{Al} + m_W c_W) \Delta T \\
    & = \qty{5.55e5}{J}
\end{align*}

\setcounter{subsubsection}{32}
\subsubsection{}

\begin{align*}
  \Delta K & = \frac{1}{2} m v^2 - \frac{1}{2} m v'^2 \\
           & = \frac{1}{2} m (v^2 - v'^2)             \\
           & = \qty{3.47}{kJ}                         \\
  \Delta K & = m c \Delta T                           \\
  \Delta T & = \frac{\Delta K}{m c}                   \\
           & = \qty{6.14e-2}{\degree C}
\end{align*}

\setcounter{subsubsection}{34}
\subsubsection{}

\begin{enumerate}
  \item

        \begin{align*}
          0   & = m_m c_m \Delta T_m + m_w c_w \Delta T_w    \\
          c_m & = -\frac{m_w c_w \Delta T_w}{m_m \Delta T_m} \\
              & = \qty{215}{J/(kg.K)}
        \end{align*}

  \item Water because it has a higher specific heat

  \item It would be too small
\end{enumerate}

\setcounter{subsubsection}{44}
\subsubsection{}

\begin{align*}
  \frac{1}{2} m v^2 & = m c \Delta T + m L_F        \\
  v                 & = \sqrt{2 (c \Delta T + L_F)} \\
                    & = \qty{366}{m/s}
\end{align*}

\setcounter{subsubsection}{54}
\subsubsection{}

\begin{align*}
  k_C A \frac{T_H - T}{L} & = k A \frac{T}{L}          \\
  k_C T_H - k_C T         & = k T                      \\
  k_C T_H                 & = (k + k_C) T              \\
  T                       & = \frac{k_C}{k + k_C} T_H  \\
  0.71                    & = \frac{k_C}{k + k_C}      \\
  0.71 (k + k_C)          & = k_C                      \\
  0.71 k + 0.71 k_C       & = k_C                      \\
  0.71 k                  & = 0.29 k_C                 \\
  k                       & = \frac{0.29}{0.71} k_C    \\
                          & \approx \qty{157}{W/(m.K)}
\end{align*}

\setcounter{subsubsection}{56}
\subsubsection{}

\begin{enumerate}
  \item

        \begin{align*}
          k_W \frac{T - T_C}{L_W}                            & = k_S \frac{T_H - T}{L_S}                                                             \\
          \left( \frac{k_W}{L_W} + \frac{k_S}{L_S} \right) T & = \frac{k_S}{L_S} T_H + \frac{k_W}{L_W} T_C                                           \\
          T                                                  & = \frac{\frac{k_S}{L_S} T_H + \frac{k_W}{L_W} T_C}{\frac{k_W}{L_W} + \frac{k_S}{L_S}} \\
                                                             & = \qty{-0.86}{\degree C}
        \end{align*}

  \item

        \begin{align*}
          H & = k_W \frac{T - T_C}{L_W} \\
            & = \qty{24.4}{W/m^2}
        \end{align*}
\end{enumerate}

\setcounter{subsubsection}{64}
\subsubsection{}

\begin{align*}
  H & = A e \sigma T^4         \\
  A & = \frac{H}{e \sigma T^4} \\
    & = \qty{2.1}{cm^2}
\end{align*}

\setcounter{subsubsection}{68}
\subsubsection{}

\begin{align*}
  \Delta L & = (\alpha_B L_B + \alpha_S L_S) \Delta T             \\
  T        & = T_0 + \frac{\Delta L}{\alpha_B L_B + \alpha_S L_S} \\
           & = \qty{35.0}{\degree C}
\end{align*}

\setcounter{subsubsection}{70}
\subsubsection{}

\begin{align*}
  Q        & = m c \Delta T                  \\
           & = \rho V c \Delta T             \\
  \Delta T & = \frac{Q}{\rho V c}            \\
  \Delta V & = \beta V \Delta T              \\
           & = \frac{\beta Q}{\rho c}        \\
  c        & = \frac{\beta Q}{\rho \Delta V}
\end{align*}

\setcounter{subsubsection}{72}
\subsubsection{}

\begin{enumerate}
  \item

        \begin{align*}
          \qty{0.0}{\degree M}                                    & = \qty{-39}{\degree C}                   \\
          \qty{100.0}{\degree M}                                  & = \qty{357}{\degree C}                   \\
          T_M                                                     & = \frac{T_C + \qty{39}{\degree C}}{3.96} \\
          \frac{\qty{100}{\degree C} + \qty{39}{\degree C}}{3.96} & = \qty{35.1}{\degree M}
        \end{align*}

  \item \[\qty{10}{M \degree} = 10 \frac{\qty{357}{\degree C} - (\qty{-39}{\degree C})}{100} = \qty{39.6}{C \degree}\]
\end{enumerate}

\setcounter{subsubsection}{74}
\subsubsection{}

\begin{align*}
  A h + \beta_G A h (T - T_0)           & = A h' + \beta_O A h' (T - T_0)                                             \\
  A h + \beta_G A h T - \beta_G A h T_0 & = A h' + \beta_O A h' T - \beta_O A h' T_0                                  \\
  (\beta_G A h - \beta_O A h') T        & = (A h' - \beta_O A h' T_0) - (A h - \beta_G A h T_0)                       \\
  T                                     & = \frac{(1 - \beta_O T_0) h' - (1 - \beta_G T_0) h}{\beta_G h - \beta_O h'} \\
                                        & = \qty{69.4}{\degree C}
\end{align*}

\setcounter{subsubsection}{78}
\subsubsection{}

\begin{enumerate}
  \item

        \begin{align*}
          Y           & = \frac{F / A}{\Delta L / L_0}                            \\
          \Delta L    & = \frac{F L_0}{A Y}                                       \\
          \Delta L    & = \alpha L_0 \Delta T                                     \\
          \Delta L    & = \alpha L_0 \Delta T + \frac{F L_0}{A Y}                 \\
          \frac{F}{A} & = Y \left( \frac{\Delta L}{L_0} - \alpha \Delta T \right)
        \end{align*}

  \item

        \begin{align*}
          \Delta L_B                & = \alpha_B L_{B0} \Delta T           \\
          \frac{\Delta L_B}{L_{B0}} & = \alpha_B \Delta T                  \\
          \frac{F}{A}               & = Y_S (\alpha_B - \alpha_S) \Delta T \\
                                    & = \qty{1.9e8}{Pa}
        \end{align*}
\end{enumerate}

\setcounter{subsubsection}{84}
\subsubsection{}

\begin{enumerate}
  \item

        \begin{align*}
          \frac{dQ}{dT} & = n k \frac{T^3}{\theta^3}                                \\
          Q             & = \int_a^b n k \frac{T^3}{\theta^3}                       \\
                        & = \frac{n k}{\theta^3} \left[ \frac{1}{4} T^4 \right]_a^b \\
                        & = \frac{n k}{4 \theta^3} (b^4 - a^4)                      \\
                        & = \qty{83.6}{J}
        \end{align*}

  \item

        \begin{align*}
          Q & = n C \Delta T          \\
          C & = \frac{Q}{n \Delta T}  \\
            & = \qty{1.86}{J/(mol.K)}
        \end{align*}

  \item \[C = \qty{5.60}{J/(mol.K)}\]
\end{enumerate}

\setcounter{subsubsection}{94}
\subsubsection{}

\begin{enumerate}
  \item

        \begin{align*}
          0 & = m_I L_f + m_I c_W \Delta T_I + m_C c_C \Delta T_I - m_S L_v + m_S c_W \Delta T_S \\
            & = m_I L_f + m_I c_W T + m_C c_C T - m_S L_v + m_S c_W (T - T_S)                    \\
          T & = \frac{m_S (L_v + c_W T_S) - m_I L_f}{m_I c_W + m_C c_C + m_S c_W}                \\
            & = \qty{86.1}{\degree C}
        \end{align*}

  \item No ice, $\qty{0.13}{kg}$ water, no steam
\end{enumerate}

\setcounter{subsubsection}{98}
\subsubsection{}

\begin{enumerate}
  \item

        \begin{align*}
          H & = k A \frac{T_H - T_C}{L} \\
            & = \qty{94}{W}
        \end{align*}

  \item

        \begin{align*}
          H_\text{wood}  & = \qty{12.4}{W}                        \\
          H_\text{glass} & = \qty{45.0}{W}                        \\
          H'             & = H + (H_\text{glass} - H_\text{wood}) \\
                         & = \qty{126.6}{W}                       \\
          \frac{H'}{H}   & = 1.35
        \end{align*}
\end{enumerate}

\setcounter{subsubsection}{104}
\subsubsection{}

\begin{enumerate}
  \setcounter{enumi}{1}
  \item

        \begin{align*}
          \frac{d Q}{d t}                 & = k \frac{T_H - T_C}{L}                        \\
          \frac{d Q}{d L}                 & = \rho L_f                                     \\
          \frac{d L}{d t}                 & = \frac{d L}{d Q} \frac{d Q}{d t}              \\
                                          & = \frac{1}{\rho L_f} k \frac{T_H - T_C}{L}     \\
          L \frac{d L}{d t}               & = \frac{k (T_H - T_C)}{\rho L_f}               \\
          \int_0^t L \frac{d L}{d t} \,dt & = \int_0^t \frac{k (T_H - T_C)}{\rho L_f} \,dt \\
          \int_0^L L' \,dL'               & = \frac{k (T_H - T_C)}{\rho L_f} t             \\
          \frac{1}{2} L^2                 & = \frac{k (T_H - T_C)}{\rho L_f} t             \\
          L                               & = \sqrt{\frac{2 k (T_H - T_C)}{\rho L_f} t}
        \end{align*}

  \item

        \begin{align*}
          t & = \frac{L^2 \rho L_f}{2 k (T_H - T_C)} \\
            & = \qty{7.5}{days}
        \end{align*}

  \item $t \approx \qty{530}{years}$; no
\end{enumerate}

\setcounter{subsubsection}{106}
\subsubsection{}

\begin{align*}
  A & = 2 \pi \left( \frac{d}{2} \right)^2 + 2 \pi \left( \frac{d}{2} \right) h \\
    & = \qty{8.34e-2}{m^2}                                                      \\
  H & = A e \sigma (T^4 - T_s^4)                                                \\
    & = A e \sigma (T^4 - T_s^4)                                                \\
    & = -\qty{3.38e-2}{W}                                                       \\
  m & = \frac{H \times 60 \times 60}{L_v}                                       \\
    & = \qty{5.82e-3}{kg/h}                                                     \\
    & = \qty{5.82}{g/h}
\end{align*}

\setcounter{subsubsection}{112}
\subsubsection{}

\begin{align*}
  r(x)                                                                             & = R_2 - (R_2 - R_1) \frac{x}{L}                                        \\
  A(x)                                                                             & = \pi r(x)^2                                                           \\
                                                                                   & = \pi \left[ R_2 - (R_2 - R_1) \frac{x}{L} \right]^2                   \\
  H                                                                                & = k A(x) \frac{d T}{d x}                                               \\
                                                                                   & = k \pi \left[ R_2 - (R_2 - R_1) \frac{x}{L} \right]^2 \frac{d T}{d x} \\
  \frac{1}{\left[ R_2 - (R_2 - R_1) \frac{x}{L} \right]^2} H \,d x                 & = k \pi \,d T                                                          \\
  \int_0^L \frac{1}{\left[ R_2 - (R_2 - R_1) \frac{x}{L} \right]^2} H \,d x        & = \int_{T_H}^{T_C} k \pi \,d T                                         \\
  \frac{H L}{R_2 - R_1} \left[ \frac{1}{R_2 - (R_2 - R_1) \frac{x}{L}} \right]_0^L & = k \pi (T_C - T_H)                                                    \\
  \frac{H L}{R_2 - R_1} \left( \frac{1}{R_1} - \frac{1}{R_2} \right)               & = k \pi (T_C - T_H)                                                    \\
  \frac{H L}{R_2 - R_1} \frac{R_2 - R_1}{R_1 R_2}                                  & = k \pi (T_C - T_H)                                                    \\
  H                                                                                & = \frac{k \pi R_1 R_2 (T_C - T_H)}{L}
\end{align*}

\setcounter{subsubsection}{114}
\subsubsection{}

\begin{enumerate}
  \item

        \begin{align*}
          H                           & = k (2 \pi r L) \frac{d T}{d r}           \\
          \frac{1}{r} H \,dr          & = 2 \pi k L \,d T                         \\
          \int_a^b \frac{1}{r} H \,dr & = \int_{T_1}^{T_2} 2 \pi k L \,d T        \\
          H \ln \frac{b}{a}           & = 2 \pi k L (T_2 - T_1)                   \\
          H                           & = \frac{2 \pi k L (T_2 - T_1)}{\ln b / a}
        \end{align*}

  \item

        \begin{align*}
          \frac{2 \pi k L (T - T_2)}{\ln r / a} & = \frac{2 \pi k L (T_2 - T_1)}{\ln b / a}       \\
          \frac{T - T_2}{\ln r / a}             & = \frac{T_2 - T_1}{\ln b / a}                   \\
          T - T_2                               & = \frac{\ln r / a}{\ln b / a} (T_2 - T_1)       \\
          T                                     & = T_2 + \frac{\ln r / a}{\ln b / a} (T_2 - T_1) \\
        \end{align*}
\end{enumerate}

\setcounter{subsubsection}{116}
\subsubsection{}

a

\setcounter{subsubsection}{118}
\subsubsection{}

a

\end{document}