\documentclass{article}
\usepackage{amsmath} % For align*
\usepackage{amsfonts} % For open face letters
\usepackage{enumitem} % For customisable list labels
\usepackage{graphicx} % For images
\usepackage{siunitx} % For units
\graphicspath{{./images/}}

\setlist[enumerate, 1]{label={(\alph*)}}
\setlist[enumerate, 2]{label={(\roman*)}}

\title{Advanced Engineering Mathematics Vectors, Matrices, and Vector Calculus by Dennis G. Zill Problems}
\author{Chris Doble}
\date{June 2023}

\begin{document}

\maketitle

\tableofcontents

\section{Vectors}

\subsection{Vectors in 2-Space}

\subsubsection{}

\begin{enumerate}
  \item $3 \mathbf{a} = 6 \mathbf{i} + 12 \mathbf{j}$

  \item $\mathbf{a} + \mathbf{b} = \mathbf{i} + 8 \mathbf{j}$

  \item $\mathbf{a} - \mathbf{b} = 3 \mathbf{i}$

  \item $||\mathbf{a} + \mathbf{b}|| = \sqrt{1 + 8^2} = \sqrt{65}$

  \item $||\mathbf{a} - \mathbf{b}|| = 3$
\end{enumerate}

\setcounter{subsubsection}{8}
\subsubsection{}

\begin{enumerate}
  \item $4 \mathbf{a} - 2 \mathbf{b} = \langle 6, -14 \rangle$

  \item $-3 \mathbf{a} - 5 \mathbf{b} = \langle 2, 4 \rangle$
\end{enumerate}

\setcounter{subsubsection}{14}
\subsubsection{}

$\overrightarrow{P_1 P_2} = \langle 2, 5 \rangle$

\setcounter{subsubsection}{18}
\subsubsection{}

$(1, 18)$

\setcounter{subsubsection}{20}
\subsubsection{}

\begin{enumerate}
  \item Yes

  \item Yes

  \item Yes

  \item No

  \item Yes

  \item Yes
\end{enumerate}

\setcounter{subsubsection}{24}
\subsubsection{}

\begin{enumerate}
  \item $\frac{\mathbf{a}}{||\mathbf{a}||} = \frac{\langle 2, 2 \rangle}{\sqrt{2^2 + 2^2}} = \frac{1}{2 \sqrt{2}} \langle 2, 2 \rangle = \langle \frac{1}{\sqrt{2}}, \frac{1}{\sqrt{2}} \rangle$

  \item $\langle -\frac{1}{\sqrt{2}}, -\frac{1}{\sqrt{2}} \rangle$
\end{enumerate}

\setcounter{subsubsection}{30}
\subsubsection{}

$2 \frac{\mathbf{a}}{||\mathbf{a}||} = 2 \frac{\langle 3, 7 \rangle}{\sqrt{3^2 + 7^2}} = \frac{2}{\sqrt{58}} \langle 3, 7 \rangle = \langle \frac{6}{\sqrt{58}}, \frac{14}{\sqrt{58}} \rangle$

\setcounter{subsubsection}{36}
\subsubsection{}

$\mathbf{x} = -(\mathbf{a} + \mathbf{b})$

\setcounter{subsubsection}{40}
\subsubsection{}

\begin{align*}
  \mathbf{a} & = 2 \mathbf{i} + 3 \mathbf{j}                                                                                     \\
  \mathbf{b} & = \mathbf{i} + \mathbf{j}                                                                                         \\
  \mathbf{c} & = \mathbf{i} - \mathbf{j}                                                                                         \\ \\
  \mathbf{i} & = \frac{1}{2} (\mathbf{b} + \mathbf{c})                                                                           \\
  \mathbf{j} & = \frac{1}{2} (\mathbf{b} - \mathbf{c})                                                                           \\
  \mathbf{a} & = 2 \left( \frac{1}{2} (\mathbf{b} + \mathbf{c}) \right) + 3 \left( \frac{1}{2} (\mathbf{b} - \mathbf{c}) \right) \\
             & = \mathbf{b} + \mathbf{c} + \frac{3}{2} \mathbf{b} - \frac{3}{2} \mathbf{c}                                       \\
             & = \frac{5}{2} \mathbf{b} - \frac{1}{2} \mathbf{c}
\end{align*}

\setcounter{subsubsection}{42}
\subsubsection{}

\begin{align*}
  y          & = \frac{1}{4} x^2 + 1                                        \\
  y(2)       & = 2                                                          \\
  y'         & = \frac{1}{2} x                                              \\
  y'(2)      & = 1                                                          \\
  \mathbf{v} & = \pm \langle \frac{1}{\sqrt{2}}, \frac{1}{\sqrt{2}} \rangle
\end{align*}

\setcounter{subsubsection}{44}
\subsubsection{}

\begin{enumerate}
  \item

        \begin{align*}
          \mathbf{F}_n                & = \mathbf{F} \cos \theta         \\
          \mathbf{F}_g                & = \mathbf{F} \sin \theta         \\
          ||\mathbf{F}_f||            & = \mu ||\mathbf{F}_n||           \\
          ||-\mathbf{F}_g||           & = \mu ||\mathbf{F}_n||           \\
          ||-\mathbf{F} \sin \theta|| & = \mu ||\mathbf{F} \cos \theta|| \\
          ||\mathbf{F}|| \sin \theta  & = \mu ||\mathbf{F}|| \cos \theta \\
          \tan \theta                 & = \mu
        \end{align*}

  \item $\theta = \arctan \mu \approx \ang{31}$
\end{enumerate}

\setcounter{subsubsection}{46}
\subsubsection{}

\begin{align*}
  F_x        & = \frac{q Q}{4 \pi \epsilon_0} \int_{-a}^a \frac{L \,dy}{2 a (L^2 + y^2)^{3 / 2}}  \\
             & = \frac{L q Q}{8 \pi \epsilon_0} \int_{-a}^a (L^2 + y^2)^{-3 / 2} \,dy             \\
             & = \frac{L q Q}{8 \pi \epsilon_0} \frac{2 a}{L^2 \sqrt{a^2 + L^2}}                  \\
             & = \frac{a q Q}{4 \pi \epsilon_0 L \sqrt{a^2 + L^2}}                                \\
  F_y        & = -\frac{q Q}{4 \pi \epsilon_0} \int_{-a}^a \frac{y \,dy}{2 a (L^2 + y^2)^{3 / 2}} \\
             & = 0                                                                                \\
  \mathbf{F} & = \langle \frac{1}{4 \pi \epsilon_0} \frac{q Q}{L \sqrt{a^2 + L^2}}, 0 \rangle
\end{align*}

\setcounter{subsubsection}{48}
\subsubsection{}

Let the three sides of the triangle be vectors $\mathbf{a}$, $\mathbf{b}$, and $\mathbf{c}$. The triangle is closed so it must be the case that \[\mathbf{a} + \mathbf{b} + \mathbf{c} = 0.\] This gives \[\mathbf{c} = -(\mathbf{a} + \mathbf{b}).\] The vector from the midpoint of side $\mathbf{a}$ to the midpoint of side $\mathbf{b}$ is \[\left( \mathbf{a} + \frac{1}{2} \mathbf{b} \right) - \frac{1}{2} \mathbf{a} = \frac{1}{2} (\mathbf{a} + \mathbf{b})\] which is parallel with $\mathbf{c}$ and half its length.

\subsection{Vectors in 3-Space}

\setcounter{subsubsection}{6}
\subsubsection{}

A plane at $z = 5$ parellel with the $x$-$y$ plane.

\setcounter{subsubsection}{8}
\subsubsection{}

A line parallel to the $z$ axis at $x = 2$ and $y = 3$.

\setcounter{subsubsection}{12}
\subsubsection{}

\begin{enumerate}
  \item $(0, 5, 4)$, $(-2, 0, 4)$, $(-2, 5, 0)$

  \item $(-2, 5, -2)$

  \item $(3, 5, 4)$
\end{enumerate}

\setcounter{subsubsection}{14}
\subsubsection{}

The planes $x = 0$, $y = 0$, and $z = 0$.

\setcounter{subsubsection}{16}
\subsubsection{}

$(-1, 2, -3)$

\setcounter{subsubsection}{18}
\subsubsection{}

The planes $z = \pm 5$.

\setcounter{subsubsection}{20}
\subsubsection{}

$\sqrt{(6 - 3)^2 + (4 + 1)^2 + (8 - 2)^2} = \sqrt{9 + 25 + 36} = \sqrt{70}$

\setcounter{subsubsection}{30}
\subsubsection{}

\begin{align*}
  \sqrt{(2 - x)^2 + (1 - 2)^2 + (1 - 3)^2} & = \sqrt{21}        \\
  (2 - x)^2 + 1 + 4                        & = 21               \\
  (2 - x)^2                                & = 16               \\
  2 - x                                    & = \pm 4            \\
  x                                        & = 2 \pm 4          \\
                                           & = -2 \text{ or } 6
\end{align*}

\setcounter{subsubsection}{32}
\subsubsection{}

$\left( 4, \frac{1}{2}, \frac{3}{2} \right)$

\setcounter{subsubsection}{36}
\subsubsection{}

$(-3, -6, 1)$

\end{document}